spatial_graph.v
@@ -3,6 +3,11 @@ Require Import overlapping.
 Require Import heap_model.
 Require Import graph.
 Require Import msl_ext.
+Require Import ramify_tactics.
+Require Import FunctionalExtensionality.
+Require Import NPeano.
+Require Import List.
+Require Import Classical.
 
 Local Open Scope pred.
 
@@ -13,8 +18,11 @@ Definition trinode x d l r :=
 
 Section SpatialGraph.
   Variable VV : Valid nat.
-  Variable pg : @PreGraph nat nat natEqDec VV.
+  Definition GV : Valid nat := fun x => VV x /\ x <> 0.
+  Variable pg : @PreGraph nat nat natEqDec GV.
   Variable bi : BiGraph pg.
+
+  Definition nodesFrom (x : adr) : list adr := @edge_func adr adr natEqDec GV pg x.
 
   Definition graph_fun (Q: adr -> pred world) (x: adr) :=
     (!!(x = 0) && emp) ||
@@ -72,21 +80,75 @@ Section SpatialGraph.
   (*   admit. *)
   (* Qed. *)
 
-  Fixpoint graphs (l : list var) :=
+  Fixpoint graphs (l : list adr) :=
     match l with
       | nil => emp
       | v :: l' => graph v ⊗ graphs l'
     end.
 
-  Fixpoint dags (l : list var) :=
+  Fixpoint dags (l : list adr) :=
     match l with
       | nil => emp
       | v :: l' => dag v ⊗ dags l'
     end.
 
-  Lemma graph_reachable_finite: forall x, graph x |-- !!(set_finite (reachable pg x)).
+  Lemma graph_path_in: forall p x y P, pg |= p is x ~o~> y satisfying P -> graph x |-- EX v : adr, (mapsto y v * TT).
   Proof.
-    repeat intro; hnf; remember (reachable pg x) as R.
+    induction p; intros; destruct H as [[? ?] [? ?]].
+    inversion H.
+    simpl in H; inversion H; subst.
+    destruct p. simpl in H0; inversion H0; subst. repeat intro.
+    rewrite graph_unfold in H3. destruct H3. destruct H3. hnf in H3; destruct H1; intuition.
+    destruct H3 as [d [l [r ?]]]. destruct_ocon H3 h. destruct_ocon H6 i.
+    destruct H10. destruct_sepcon H12 j. destruct_sepcon H13 k. exists d.
+    try_join k2 j2 m1; try_join m1 i3 m2; try_join m2 h3 m3. exists k1, m3; split; auto.
+
+    assert (pg |= n :: p is n ~o~> y satisfying P).
+    split; [split; [simpl; auto | auto] | split; [destruct H1; auto | repeat intro; apply H2; apply in_cons; auto]].
+
+    repeat intro; hnf.
+    rewrite graph_unfold in H4. destruct H4. destruct H4; hnf in H4; destruct H1; destruct H1; destruct H1; intuition.
+    destruct H4 as [d [l [r ?]]].
+    destruct_ocon H4 h. destruct_ocon H7 i. destruct H11 as [[? ?] ?].
+    unfold gamma in H11.
+    destruct_sepcon H14 j. destruct_sepcon H15 k. destruct H1 as [[? [? ?]] ?].
+    revert H11. case_eq (biEdge bi x); intros.
+    inversion H22; subst.
+    generalize (biEdge_only2 bi _ _ _ _ H11 H20); intros.
+    destruct H23; subst.
+    specialize (IHp _ _ _ H3 _ H12). hnf in IHp. simpl in IHp.
+    destruct IHp as [bb ?]. exists bb. apply join_sub_mapsto with i23; auto.
+    try_join i2 i3 i23'; equate_join i23 i23'.
+    assertSub i23 a S3; trivial.
+    specialize (IHp _ _ _ H3 _ H8). hnf in IHp. simpl in IHp.
+    destruct IHp as [bb ?]. exists bb. apply join_sub_mapsto with h23; auto.
+    try_join h2 h3 h23'; equate_join h23 h23'.
+    assertSub h23 a S1; trivial.
+  Qed.
+
+  Lemma graph_reachable_in: forall x y, reachable pg x y -> graph x |-- EX v : adr, (mapsto y v * TT).
+  Proof. intros; destruct H; apply graph_path_in in H; trivial. Qed.
+
+  Definition explode (x : adr) (w : world) (H : (graph x * TT)%pred w) :
+    {l : adr & {r : adr | biEdge bi x = (l, r) /\ valid x /\ (graph l * TT)%pred w /\ (graph r * TT)%pred w}} + {x = 0}.
+    destruct (eq_nat_dec x 0). right; auto. left.
+    rewrite graph_unfold in H.
+    assert (S : ((EX  d : adr,
+                         (EX  l : adr,
+                                  (EX  r : adr,
+                                           !!(gamma bi x = (d, l, r) /\ valid x) && trinode x d l r
+                                             ⊗ graph l ⊗ graph r))) * TT)%pred w).
+    destruct_sepcon H h. hnf in H0. destruct H0. destruct H0. hnf in H0. exfalso; auto.
+    exists h1, h2; split; auto. clear H. remember (gamma bi x). destruct p as [[d l] r]. exists l, r.
+    destruct_sepcon S h. destruct H0 as [dd [ll [rr ?]]]. destruct_ocon H0 i. destruct_ocon H4 j.
+    destruct H8 as [[? ?] ?]. injection H8; intros; subst; clear H8. unfold gamma in Heqp. destruct (biEdge bi x).
+    injection Heqp; intros; subst; clear Heqp. repeat split; auto.
+    try_join j2 j3 j23'. equate_join j23 j23'. try_join j1 i3 j1i3. try_join j1i3 h2 j1i3h2. exists j23, j1i3h2.
+    repeat split; auto. try_join i2 i3 i23'; equate_join i23 i23'. try_join i1 h2 i1h2. exists i23, i1h2. repeat split; auto.
+  Defined.
+    
+  Lemma graph_reachable_finite: forall x w, x <> 0 -> graph x w -> set_finite (reachable pg x).
+  Proof.
     admit.
   Qed.
 
