make_ramify.sh
@@ -1,8 +1,8 @@
 coqc graph.v
 coqc ramify_tactics.v
 coqc msl_ext.v
-coqc heap_model.v
 coqc overlapping.v
 coqc ramification.v
+coqc heap_model.v
 # coqc dag.v
-# coqc spatial_graph.v
+coqc spatial_graph.v
